wip on putting map library into automatable shape, but
Existing Instance map_domain_set.
Existing Instance map_range_set.

is a bad idea because different places will use different set instances, same for

Existing Instance set_elem_eq_dec.

(see PROBLEM comments)

compiler/src/StateCalculus.v
@@ -7,37 +7,13 @@ Require Import lib.fiat_crypto_tactics.UniquePose.
 
 Section StateCalculus.
 
-  Context {var: Type}. (* variable name (key) *)
-  Context {dec_eq_var: DecidableEq var}.
-  Context {val: Type}. (* value *)
-  Context {dec_eq_val: DecidableEq val}.
+  Context {var val: Type}.
   Context {stateMap: MapFunctions var val}.
-  Notation state := (map var val).
-  Context {eq_var_dec: DecidableEq var}.
-  Context {varset: SetFunctions var}.
-  Notation vars := (set var).
 
-  Definition extends(s1 s2: state) := forall x w, get s2 x = Some w -> get s1 x = Some w.
-
-  Definition only_differ(s1: state)(vs: vars)(s2: state) :=
-    forall x, x \in vs \/ get s1 x = get s2 x.
-
-  Definition agree_on(s1: state)(vs: vars)(s2: state) :=
-    forall x, x \in vs -> get s1 x = get s2 x.
-
-  Definition undef(s: state)(vs: vars) := forall x, x \in vs -> get s x = None.
-
-  Lemma get_put: forall (s: state) (x y: var) (v: val),
-    get (put s x v) y = if dec (x = y) then Some v else get s y.
-  Proof.
-    intros. destruct (dec (x = y)).
-    - subst. rewrite get_put_same. reflexivity.
-    - rewrite get_put_diff by assumption. reflexivity.
-  Qed.
-  
-  Lemma only_differ_putmany : forall (bs : list var) (vs : list val) st st' 
+  Lemma only_differ_putmany : forall (bs : list var) (vs : list val) st st'
                                      (H : putmany bs vs st = Some st'),
       only_differ st (fold_right union empty_set (List.map singleton_set bs)) st'.
+  Proof.
     induction bs, vs; cbn; try discriminate.
     { inversion 1; subst. cbv; eauto. }
     { intros ? ? H; destruct (putmany bs vs st) eqn:Heqo; [|discriminate].
@@ -47,9 +23,10 @@ Section StateCalculus.
         autorewrite with rew_set_op_specs in *; rewrite ?get_put;
           destruct (dec (a=x)); eauto. }
   Qed.
+
 End StateCalculus.
 
-Hint Unfold extends only_differ agree_on undef : unf_state_calculus.
+Hint Unfold extends only_differ agree_on undef_on : unf_state_calculus.
 
 Ltac rewrite_get_put :=
   rewrite? get_put in *;
