compiler/src/util/Map.v
@@ -82,3 +82,135 @@ Class MapFunctions(K V: Type) := mkMap {
 }.
 
 Arguments map _ _ {_}.
+
+Existing Instance map_domain_set.
+Existing Instance map_range_set.
+
+Section MapDefinitions.
+
+  Context {K V: Type}.
+  Context {KVmap: MapFunctions K V}.
+
+  Definition extends(s1 s2: map K V) := forall x w, get s2 x = Some w -> get s1 x = Some w.
+
+  Definition only_differ(s1: map K V)(vs: set K)(s2: map K V) :=
+    forall x, x \in vs \/ get s1 x = get s2 x.
+
+  Definition agree_on(s1: map K V)(vs: set K)(s2: map K V) :=
+    forall x, x \in vs -> get s1 x = get s2 x.
+
+  Definition undef_on(s: map K V)(vs: set K) := forall x, x \in vs -> get s x = None.
+
+  Lemma get_put: forall (s: map K V) (x y: K) (v: V),
+    get (put s x v) y = if dec (x = y) then Some v else get s y.
+  Proof.
+    intros. destruct (dec (x = y)).
+    - subst. rewrite get_put_same. reflexivity.
+    - rewrite get_put_diff by assumption. reflexivity.
+  Qed.
+
+  Lemma get_remove: forall (m: map K V) (x y: K),
+    get (remove m x) y = if dec (x = y) then None else get m y.
+  Proof.
+    intros. destruct (dec (x = y)).
+    - subst. rewrite get_remove_same. reflexivity.
+    - rewrite get_remove_diff by assumption. reflexivity.
+  Qed.
+
+  Lemma get_restrict: forall m k ks,
+      get (restrict m ks) k = if dec (k \in ks) then get m k else None.
+  Proof.
+    intros. destruct (dec (k \in ks)).
+    - subst. rewrite get_restrict_in; auto.
+    - rewrite get_restrict_notin by assumption. reflexivity.
+  Qed.
+
+  Lemma get_intersect_map: forall k m1 m2,
+      get (intersect_map m1 m2) k =
+      match get m1 k, get m2 k with
+      | Some v1, Some v2 => if dec (v1 = v2) then Some v1 else None
+      | _, _ => None
+      end.
+  Proof.
+    intros.
+    destruct (get (intersect_map m1 m2) k) eqn: E.
+    - apply intersect_map_spec in E. destruct E as [E1 E2].
+      rewrite E1. rewrite E2. destruct (dec (v = v)); congruence.
+    - destruct (get m1 k) eqn: E1; destruct (get m2 k) eqn: E2; auto.
+      destruct (dec (v = v0)); auto.
+      subst v0.
+      pose proof (intersect_map_spec k v m1 m2) as P.
+      firstorder congruence.
+  Qed.
+
+  Lemma get_remove_keys: forall m k ks,
+      get (remove_keys m ks) k =
+      match get m k with
+      | Some v => if dec (k \in ks) then None else Some v
+      | None => None
+      end.
+  Proof.
+    intros.
+    destruct (get m k) eqn: E.
+    - destruct (dec (k \in ks)).
+      + eauto using remove_keys_removed.
+      + eauto using remove_keys_not_removed.
+    - eauto using remove_keys_never_there.
+  Qed.
+
+  Lemma get_remove_by_value: forall m k v,
+      get (remove_by_value m v) k =
+      if dec (get m k = Some v) then None else get m k.
+  Proof.
+    intros. destruct (dec (get m k = Some v)).
+    - eauto using remove_by_value_same.
+    - eauto using remove_by_value_diff.
+  Qed.
+
+  Lemma get_remove_values: forall m k vs,
+      get (remove_values m vs) k =
+      match get m k with
+      | Some v => if dec (v \in vs) then None else Some v
+      | None => None
+      end.
+  Proof.
+    (*
+  remove_values: map -> set V -> map;
+  remove_values_never_there: forall m k vs,
+      get m k = None ->
+      get (remove_values m vs) k = None;
+  remove_values_removed: forall m k v vs,
+      get m k = Some v ->
+      v \in vs ->
+      get (remove_values m vs) k = None;
+  remove_values_not_removed: forall m k v vs,
+      get m k = Some v ->
+      ~ v \in vs ->
+      get (remove_values m vs) k = Some v;
+
+  update_map: map -> map -> map;
+  get_update_map_l: forall m1 m2 k,
+      get m2 k = None ->
+      get (update_map m1 m2) k = get m1 k;
+  get_update_map_r: forall m1 m2 k v,
+      get m2 k = Some v ->
+      get (update_map m1 m2) k = Some v;
+*)
+  Abort.
+
+
+End MapDefinitions.
+
+Hint Unfold extends only_differ agree_on undef_on : unf_map_defs.
+
+Hint Rewrite
+     @get_remove
+     @get_put
+
+
+     @domain_spec
+     @range_spec
+
+  (* TODO operations without a rewrite lemma here:
+     - reverse_get
+  *).
